Filrb/Internal/Invariants/RBInv.lean
@@ -1,0 +1,161 @@
+import Filrb.Internal.Raw
+import Filrb.Internal.Invariants.BST
+
+/-!
+This module proves that our functionality preserves the `RedBlackTree` invariant,
+which is a combination of the `ChildInv` and the `HeightInv` invariant.
+-/
+
+namespace Filrb
+namespace Internal
+
+namespace Raw
+
+variable [Preorder α] [Ord α] [LawfulOrd α]
+
+/--
+The child invariant for red black trees: Red nodes must have black children.
+-/
+inductive ChildInv : Raw α → Prop where
+  | nil : ChildInv .nil
+  | black (hleft : ChildInv left) (hright : ChildInv right) : ChildInv (.node left data .black right)
+  | red (hleft1 : ChildInv left) (hleft2 : left.rootColor = .black) (hright1 : ChildInv right)
+        (hright2 : right.rootColor = .black) : ChildInv (.node left data .red right)
+
+attribute [pp_nodot] ChildInv
+
+/--
+A weaker child invariant for red black trees,
+where only the childs of a node have to preserve the invariant.
+-/
+def ChildInv2 (t : Raw α) : Prop :=
+  ChildInv (paintColor .black t)
+
+attribute [pp_nodot] ChildInv2
+
+omit [Preorder α] [Ord α] [LawfulOrd α] in
+@[simp]
+theorem childInv_nil : ChildInv (.nil : Raw α) := ChildInv.nil
+
+omit [Preorder α] [Ord α] [LawfulOrd α] in
+@[simp]
+theorem childInv2_nil : ChildInv2 (.nil : Raw α) := ChildInv.nil
+
+omit [Preorder α] [Ord α] [LawfulOrd α] in
+@[simp]
+theorem childInv_red_node {l r : Raw α} :
+    ChildInv (.node l d .red r) ↔ ChildInv l ∧ (l.rootColor = .black) ∧ ChildInv r ∧ (r.rootColor = .black) := by
+  constructor
+  · intro h
+    cases h
+    simp_all
+  · rintro ⟨_, _, _, _⟩
+    apply ChildInv.red <;> assumption
+
+omit [Preorder α] [Ord α] [LawfulOrd α] in
+@[simp]
+theorem childInv_black_node {l r : Raw α} :
+    ChildInv (.node l d .black r) ↔ ChildInv l ∧ ChildInv r := by
+  constructor
+  · intro h
+    cases h
+    simp_all
+  · rintro ⟨_, _⟩
+    apply ChildInv.black <;> assumption
+
+omit [Preorder α] [Ord α] [LawfulOrd α] in
+@[aesop safe forward]
+theorem childInv_node {l r : Raw α} (h : ChildInv (.node l d c r)) :
+    ChildInv l ∧ ChildInv r := by
+  rcases h <;> simp_all
+
+omit [Preorder α] [Ord α] [LawfulOrd α] in
+theorem childInv_color_independent {l r : Raw α} (h : ChildInv (.node l d c r)) :
+    ChildInv (.node l d .black r) := by
+  rw [childInv_black_node]
+  apply childInv_node h
+
+omit [Preorder α] [Ord α] [LawfulOrd α] in
+theorem childInv_paintColorBlack_of_childInv (t : Raw α) (h : ChildInv t) :
+    ChildInv (t.paintColor .black) := by
+  unfold paintColor
+  split <;> aesop
+
+@[aesop safe apply]
+theorem childInv2_of_childInvL (hl : ChildInv l) (hr : ChildInv r) :
+    ChildInv2 (.node l d c r) := by
+  simp [ChildInv2, paintColor, hl, hr]
+
+def blackHeightLeft (t : Raw α) : Nat :=
+  match t with
+  | .nil => 0
+  | .node left _ color _ =>
+    match color with
+    | .black => blackHeightLeft left + 1
+    | .red => blackHeightLeft left
+
+/--
+The height invariant for red black trees: Every path from a given node to any of its leaves goes
+through the same number of black nodes.
+
+The particular variant here is based on
+[Functional Algorithms Verified](https://functional-algorithms-verified.org/functional_data_structures_algorithms.pdf)
+and uses a sufficient condition instead of directly encoding the above.
+-/
+inductive HeightInv : Raw α → Prop where
+  | nil : HeightInv .nil
+  | node (hleft : HeightInv left) (hright : HeightInv right)
+         (h : left.blackHeightLeft = right.blackHeightLeft) : HeightInv (.node left data color right)
+
+attribute [pp_nodot] HeightInv
+
+omit [Preorder α] [Ord α] [LawfulOrd α] in
+@[simp]
+theorem heightInv_nil : HeightInv (.nil : Raw α) := HeightInv.nil
+
+theorem rbInv_insert_of_rbInv (x : α) (t : Raw α) (hc : ChildInv t) (hh : HeightInv t) :
+    ChildInv (t.insert x) ∧ HeightInv (t.insert x) := by
+  sorry
+
+theorem rbInv_baldL_of_rbInv {x : α} {l r t : Raw α}
+    (hcl : ChildInv2 l) (hcr : ChildInv r)
+    (hhl : HeightInv l) (hhr : HeightInv r)
+    (hbh : blackHeightLeft l + 1 = blackHeightLeft r) (heq : baldL x l r = t) :
+    (if r.isBlack then ChildInv t ∧ ChildInv2 t else ChildInv2 t)
+    ∧ HeightInv t ∧ blackHeightLeft t = blackHeightLeft r := by
+  sorry
+
+theorem rbInv_baldR_of_rbInv {x : α} {l r t : Raw α}
+    (hcl : ChildInv l) (hcr : ChildInv2 r)
+    (hhl : HeightInv l) (hhr : HeightInv r)
+    (hbh : blackHeightLeft l = blackHeightLeft r + 1) (heq : baldR x l r = t) :
+    (if l.isBlack then ChildInv t ∧ ChildInv2 t else ChildInv2 t)
+    ∧ HeightInv t ∧ blackHeightLeft t = blackHeightLeft l := by
+  sorry
+
+-- 8.1 has a requirement that for `split_min t = (x,t')` t has to be not nil?
+theorem rbInv_appendTrees_of_rbInv {l r t : Raw α} (hc : ChildInv (.node l d c r))
+    (hh : HeightInv (.node l d c r)) (heq : appendTrees l r = t) :
+    (if c = .black then
+      blackHeightLeft t = blackHeightLeft l - 1 ∧ ChildInv2 t
+    else
+      blackHeightLeft t = blackHeightLeft l ∧ ChildInv t)
+    ∧ HeightInv t' := by
+  sorry
+
+theorem rbInv_del_of_rbInv {t t' : Raw α}
+    (hc : ChildInv t) (hh : HeightInv t) (heq : del x t = t') :
+    (if t.isBlack then
+      blackHeightLeft t' = blackHeightLeft t - 1 ∧ ChildInv2 t'
+    else
+      blackHeightLeft t' = blackHeightLeft t ∧ ChildInv t')
+    ∧ HeightInv t' := by
+  sorry
+
+theorem rbInv_erase_of_rbInv (x : α) (t : Raw α) (hc : ChildInv t) (hh : HeightInv t) :
+    ChildInv (t.erase x) ∧ HeightInv (t.erase x) := by
+  sorry
+
+end Raw
+end Internal
+end Filrb
